feat(data/finset): max and min

data/finset.lean
@@ -1043,6 +1043,72 @@ by haveI := classical.prop_decidable;
 
 end fold
 
+/- max and min of finite sets -/
+section max_min
+variables [decidable_linear_order α]
+
+def max (a : α) : finset α → α :=
+fold _root_.max a id
+
+@[simp] theorem max_empty {a : α} : max a (∅ : finset α) = a :=
+by simp [max]
+
+@[simp] theorem max_insert {a b : α} {s : finset α} (h : a ∉ s) :
+  max b (insert a s) = _root_.max a (max b s) :=
+by simp [max, fold_insert h]
+
+@[simp] theorem max_singleton {a b : α} : max b {a} = _root_.max a b :=
+by simp [max]
+
+theorem le_max_left (a : α) (s : finset α) : a ≤ max a s :=
+finset.induction_on s
+  (by rw max_empty)
+  (λ b s (hnm : b ∉ s) (ih : a ≤ max a s),
+   by rw max_insert hnm; exact le_trans ih (le_max_right b (max a s)))
+
+theorem le_max_of_mem {a b : α} {s : finset α} (h : a ≤ b) : a ∈ s → a ≤ max b s :=
+finset.induction_on s
+  (λ _, by simp only [max_empty, h])
+  (λ c s (hnm : c ∉ s) (ih : a ∈ s → a ≤ max b s) (hins : a ∈ insert c s),
+   begin
+     rw max_insert hnm,
+     cases mem_insert.mp hins,
+     case or.inl : p { simp only [p, _root_.le_max_left] },
+     case or.inr : p { exact le_trans (ih p) (le_max_right c (max b s)) }
+   end)
+
+def min (a : α) : finset α → α :=
+fold _root_.min a id
+
+@[simp] theorem min_empty {a : α} : min a (∅ : finset α) = a :=
+by simp [min]
+
+@[simp] theorem min_insert {a b : α} {s : finset α} (h : a ∉ s) :
+  min b (insert a s) = _root_.min a (min b s) :=
+by simp [min, fold_insert h]
+
+@[simp] theorem min_singleton {a b : α} : min b {a} = _root_.min a b :=
+by simp [min]
+
+theorem min_le_left (a : α) (s : finset α) : min a s ≤ a :=
+finset.induction_on s
+  (by rw min_empty)
+  (λ b s (hnm : b ∉ s) (ih : min a s ≤ a),
+   by rw min_insert hnm; exact le_trans (min_le_right b (min a s)) ih)
+
+theorem min_le_of_mem {a b : α} {s : finset α} (h : a ≤ b) : b ∈ s → min a s ≤ b :=
+finset.induction_on s
+  (λ _, by simp only [min_empty, h])
+  (λ c s (hnm : c ∉ s) (ih : b ∈ s → min a s ≤ b) (hins : b ∈ insert c s),
+   begin
+     rw min_insert hnm,
+     cases mem_insert.mp hins,
+     case or.inl : p { simp only [p, _root_.min_le_left] },
+     case or.inr : p { exact le_trans (min_le_right c (min a s)) (ih p) }
+   end)
+
+end max_min
+
 section sort
 variables (r : α → α → Prop) [decidable_rel r]
   [is_trans α r] [is_antisymm α r] [is_total α r]
